imp/Imp.v
@@ -90,11 +90,12 @@ Record program : Type := mk_program {
   prog_vars : progVars;
   prog_funs : progFuns;
   public : list gname :=
+    let sys := List.map fst syscalls in
     let evs := ext_vars in
-    let efs := List.map (fun p => fst p) ext_funs in
-    let ivs := List.map (fun p => fst p) prog_vars in
-    let ifs := List.map (fun p => fst p) prog_funs in
-    ["malloc"; "free"] ++ evs ++ efs ++ ivs ++ ifs;
+    let efs := List.map fst ext_funs in
+    let ivs := List.map fst prog_vars in
+    let ifs := List.map fst prog_funs in
+    ["malloc"; "free"] ++ sys ++ evs ++ efs ++ ivs ++ ifs;
   defs : list (gname * Sk.gdef) :=
     let fs := (List.map (fun '(fn, _) => (fn, Sk.Gfun)) prog_funs) in
     let vs := (List.map (fun '(vn, vv) => (vn, Sk.Gvar vv)) prog_vars) in
